theories/term.v
@@ -23,7 +23,7 @@ Inductive Term : Type :=
 | app : Term -> Term -> Term
 | const : Constant -> Term
 | var : string -> nat -> Term (*nth variable with that name, going up like debruin indices*)
-| lift : string -> Term -> Term
+| lift : string -> nat -> Term -> Term
 (* the var info, the term being subbed for the var, the term being subbed into *)
 | subst : string -> nat -> Term -> Term -> Term.
 
@@ -37,13 +37,13 @@ Inductive convertible : Term -> Term -> Prop :=
 | beta : forall {s t1 t2}, convertible (app (lam s t1) t2) (subst s 0 t2 t1)
 | betapi1 : forall {t1 t2}, convertible (pi1 (pair t1 t2)) t1
 | betapi2 : forall {t1 t2}, convertible (pi2 (pair t1 t2)) t2
-| eta : forall {s t}, convertible t (lam s (app (lift s t) (var s 0)))
+| eta : forall {s t}, convertible t (lam s (app (lift s 0 t) (var s 0)))
 | SP : forall {t}, convertible t (pair (pi1 t) (pi2 t))
 (* congruence convertibles *)
 | lam_cong : forall s t t', convertible t t' -> convertible (lam s t) (lam s t')
 | app_cong : forall t1 t1' t2 t2',
     convertible t1 t1' -> convertible t2 t2' -> convertible (app t1 t2) (app t1' t2')
-| lift_cong : forall s t t', convertible t t' -> convertible (lift s t) (lift s t')
+| lift_cong : forall s i t t', convertible t t' -> convertible (lift s i t) (lift s i t')
 | subst_cong : forall s i t1 t1' t2 t2',
     convertible t1 t1' -> convertible t2 t2'
     -> convertible (subst s i t1 t2) (subst s i t1' t2')
@@ -52,30 +52,31 @@ Inductive convertible : Term -> Term -> Prop :=
 | conv_trans : forall t1 t2 t3, convertible t1 t2 -> convertible t2 t3 -> convertible t1 t3
 | conv_sym : forall t1 t2, convertible t1 t2 -> convertible t2 t1
 (* small step substitution and lifting *)
-| lift_app : forall s t1 t2, convertible (lift s (app t1 t2)) (app (lift s t1) (lift s t2))
-| lift_lam : forall s1 s2 t, convertible (lift s1 (lam s2 t)) (lam s2 (lift s1 t))
+| lift_app : forall s i t1 t2, convertible (lift s i (app t1 t2)) (app (lift s i t1) (lift s i t2))
+| lift_lam : forall s1 i s2 t,
+    convertible (lift s1 i (lam s2 t)) (lam s2 (lift s1 (if eqb s1 s2 then S i else i) t))
 (* TODO: Surely this is wrong? Shouldn't it compare the two indices? In fact, shouldn't 
 lift TAKE an index? Check Nipkow paper. *)
-| lift_var : forall (s1 s2 : string) (i : nat),
-    convertible (lift s1 (var s2 i))
-      (if String.eqb s1 s2
+| lift_var : forall (s1 s2 : string) (i k : nat),
+    convertible (lift s1 k (var s2 i))
+      (if andb (String.eqb s1 s2) (negb (Nat.ltb i k))
       then var s2 (S i)
        else var s2 i)
-| lift_const : forall s1 s2, convertible (lift s1 (const s2)) (const s2)
+| lift_const : forall s1 i s2, convertible (lift s1 i (const s2)) (const s2)
 | subst_app : forall s i t t1 t2,
     convertible (subst s i t (app t1 t2)) (app (subst s i t t1) (subst s i t t2))
 (* Is this right now? *)
 | subst_lam : forall s1 s2 i t1 t2,
     convertible (subst s2 i t2 (lam s1 t1))
                 (if String.eqb s1 s2
-                 then lam s1 (subst s2 (S i) (lift s1 t2) t1)
-                 else lam s1 (subst s2 i (lift s1 t2) t1))
+                 then lam s1 (subst s2 (S i) (lift s1 0 t2) t1)
+                 else lam s1 (subst s2 i (lift s1 0 t2) t1))
 | subst_var : forall x y n i toSub, convertible (subst x i toSub (var y n))
     (if andb (String.eqb y x) (Nat.eqb n i) then toSub else var y n)
 | subst_const : forall s1 s2 i t, convertible (subst s1 i t (const s2)) (const s2)
 (* extra facts *)
 | subst_id : forall s i t, convertible (subst s i (var s i) t) t
-| subst_lift : forall s t1 t2, convertible (subst s 0 t1 (lift s t2)) t2
+| subst_lift : forall s i t1 t2, convertible (subst s i t1 (lift s i t2)) t2
 (*| subst_subst : forall s1 i1 t1 s2 i2 t2 t,
     convertible (subst s1 i1 t1 (subst s2 i2 t2 t)) (subst s2 ????*)
 (* lift_lift ???*)                                           
